doc/oopsla21/supplement/readme.txt
@@ -1,0 +1,45 @@
+This folder contains supplementry material associated with
+the paper Union Types with Disjoint Switches.
+
+Each folder contains Coq files for a variant of
+our calculus. Organization of folders is:
+
+|------------------|------------------------------------------------|--------------------------|
+|  Folder          |   Systam                                       | Reference in paper       |
+|------------------|------------------------------------------------|--------------------------|
+|union             | Union calculus                                 | Discussed in section 3   |
+|------------------|------------------------------------------------|--------------------------|
+|union-inter       | Union calculus with intersection types         | Discussed in section 4   |
+|------------------|------------------------------------------------|--------------------------|
+|general-subtyping | Union calculus with generalized subtyping rule | Discussed in section 5.1 |
+|------------------|------------------------------------------------|--------------------------|
+|distributivity    | Union calculus with distributive subtyping     | Discussed in section 5.2 |
+|------------------|------------------------------------------------|--------------------------|
+
+
+Each folder further has two files, namely syntax.v and typing.v.
+
+------
+syntax:
+------
+This file defines syntax of the calculus and disjointness properties
+
+-------
+typing:
+-------
+This file contains semantics and properties related to type-safety.
+typing.v depends upon syntax.v.
+
+------------
+Dependencies
+------------
+
+
+Coq Version:
+-----------
+We used Coq version 8.10.0 in our development
+
+
+External Library:
+----------------
+TLC library is required to run the files.
